Updates.

HandbookOfPracticalLogicLean/Prop/Unification/Equation.lean
@@ -2,6 +2,8 @@ import HandbookOfPracticalLogicLean.Prop.Replace.Var.One.Rec.Replace
 import HandbookOfPracticalLogicLean.Prop.Size
 import HandbookOfPracticalLogicLean.Prop.Var
 
+import MathlibExtraLean.List
+
 
 set_option autoImplicit false
 
@@ -47,45 +49,25 @@ def equation_list_formula_list
 #eval equation_list_formula_list [⟨var_ "P", var_ "Q"⟩, ⟨var_ "R", var_ "S"⟩]
 
 
-lemma mem_equation_list_formula_list_imp_exists_mem_equation_list
+/--
+  `formula_occurs_in_equation_list F ES` := True if and only if there is an occurrence of the formula `F` in the list of equations `ES`.
+-/
+def formula_occurs_in_equation_list
   (F : Formula_)
-  (ES : List Equation)
-  (h1 : F ∈ equation_list_formula_list ES) :
-  ∃ (E : Equation), E ∈ ES ∧ (F = E.lhs ∨ F = E.rhs) :=
-  by
-  unfold equation_list_formula_list at h1
-  induction ES
-  case nil =>
-    simp only [List.foldr_nil, List.not_mem_nil] at h1
-  case cons hd tl ih =>
-    simp only [List.foldr_cons, List.mem_cons] at h1
+  (ES : List Equation) :
+  Prop :=
+  ∃ (E : Equation), E ∈ ES ∧ (F = E.lhs ∨ F = E.rhs)
 
-    simp only [List.mem_cons]
-    cases h1
-    case inl h1 =>
-      apply Exists.intro hd
-      constructor
-      · left
-        rfl
-      · left
-        exact h1
-    case inr h1 =>
-      cases h1
-      case inl h1 =>
-        apply Exists.intro hd
-        constructor
-        · left
-          rfl
-        · right
-          exact h1
-      case inr h1 =>
-        specialize ih h1
-        obtain ⟨E, ih_left, ih_right⟩ := ih
-        apply Exists.intro E
-        constructor
-        · right
-          exact ih_left
-        · exact ih_right
+instance
+  (F : Formula_)
+  (ES : List Equation) :
+  Decidable (formula_occurs_in_equation_list F ES) :=
+  by
+  unfold formula_occurs_in_equation_list
+  infer_instance
+
+
+-------------------------------------------------------------------------------
 
 
 lemma mem_equation_list_imp_mem_equation_list_formula_list_left
@@ -143,14 +125,55 @@ lemma mem_equation_list_imp_mem_equation_list_formula_list_right
       exact h1
 
 
-lemma mem_equation_list_formula_list_iff_exists_mem_equation_list
+lemma mem_equation_list_formula_list_imp_formula_occurs_in_equation_list
+  (F : Formula_)
+  (ES : List Equation)
+  (h1 : F ∈ equation_list_formula_list ES) :
+  formula_occurs_in_equation_list F ES :=
+  by
+  unfold equation_list_formula_list at h1
+
+  unfold formula_occurs_in_equation_list
+  induction ES
+  case nil =>
+    simp only [List.foldr_nil, List.not_mem_nil] at h1
+  case cons hd tl ih =>
+    simp only [List.foldr_cons, List.mem_cons] at h1
+
+    simp only [List.mem_cons]
+    cases h1
+    case inl h1 =>
+      apply Exists.intro hd
+      constructor
+      · left
+        rfl
+      · left
+        exact h1
+    case inr h1 =>
+      cases h1
+      case inl h1 =>
+        apply Exists.intro hd
+        constructor
+        · left
+          rfl
+        · right
+          exact h1
+      case inr h1 =>
+        specialize ih h1
+        obtain ⟨E, ih_left, ih_right⟩ := ih
+        apply Exists.intro E
+        constructor
+        · right
+          exact ih_left
+        · exact ih_right
+
+
+lemma formula_occurs_in_equation_list_iff_mem_equation_list_formula_list
   (F : Formula_)
   (ES : List Equation) :
-  F ∈ equation_list_formula_list ES ↔
-    ∃ (E : Equation), E ∈ ES ∧ (F = E.lhs ∨ F = E.rhs) :=
+  formula_occurs_in_equation_list F ES ↔ F ∈ equation_list_formula_list ES :=
   by
   constructor
-  · apply mem_equation_list_formula_list_imp_exists_mem_equation_list
   · intro a1
     obtain ⟨E, a1_left, a1_right⟩ := a1
     cases a1_right
@@ -162,6 +185,18 @@ lemma mem_equation_list_formula_list_iff_exists_mem_equation_list
       rewrite [a1_right]
       apply mem_equation_list_imp_mem_equation_list_formula_list_right
       exact a1_left
+  · apply mem_equation_list_formula_list_imp_formula_occurs_in_equation_list
+
+
+-------------------------------------------------------------------------------
+
+
+lemma formula_occurs_in_equation_list_iff_mem_equation_list_formula_set
+  (F : Formula_)
+  (ES : List Equation) :
+  formula_occurs_in_equation_list F ES ↔ F ∈ equation_list_formula_set ES :=
+  by
+  sorry
 
 
 -------------------------------------------------------------------------------
@@ -186,12 +221,37 @@ def Equation.var_list
 
 
 /--
+  `var_occurs_in_equation V E` := True if and only if there is an occurrence of the variable `V` in the equation `E`.
+-/
+def var_occurs_in_equation
+  (V : String)
+  (E : Equation) :
+  Prop :=
+  var_occurs_in_formula V E.lhs ∨ var_occurs_in_formula V E.rhs
+
+instance
+  (V : String)
+  (E : Equation) :
+  Decidable (var_occurs_in_equation V E) :=
+  by
+  unfold var_occurs_in_equation
+  infer_instance
+
+
+-- lemma var_occurs_in_equation_iff_mem_equation_var_set
+
+-- lemma var_occurs_in_equation_iff_mem_equation_var_list
+
+-------------------------------------------------------------------------------
+
+/--
   `equation_list_var_set ES` := The set of all of the variables that have an occurrence in the list of equations `ES`.
 -/
 def equation_list_var_set
   (ES : List Equation) :
   Finset String :=
-  formula_list_var_set (equation_list_formula_list ES)
+  List.foldr (fun (next : Equation) (prev : Finset String) => next.var_set ∪ prev) {} ES
+  -- formula_list_var_set (equation_list_formula_list ES)
 
 #eval equation_list_var_set {}
 #eval equation_list_var_set [⟨var_ "P", var_ "Q"⟩]
@@ -205,31 +265,23 @@ def equation_list_var_set
 def equation_list_var_list
   (ES : List Equation) :
   List String :=
-  formula_list_var_list (equation_list_formula_list ES)
+  List.foldr (fun (next : Equation) (prev : List String) => next.var_list ++ prev) [] ES
+  -- formula_list_var_list (equation_list_formula_list ES)
 
 
-example
+def var_occurs_in_equation_list
   (X : String)
   (ES : List Equation) :
-  X ∈ equation_list_var_set ES ↔ ∃ (F : Formula_), F ∈ equation_list_formula_list ES ∧ X ∈ F.var_set :=
-  by
-  unfold equation_list_var_set
-  simp only [← var_occurs_in_formula_list_iff_mem_formula_list_var_set]
-  unfold var_occurs_in_formula_list
-  simp only [var_occurs_in_formula_iff_mem_formula_var_set]
+  Prop :=
+  ∃ (E : Equation), E ∈ ES ∧ var_occurs_in_equation X E
 
 
-lemma equation_list_var_set_cons
-  (E : Equation)
-  (ES : List Equation) :
-  equation_list_var_set (E :: ES) =
-    E.var_set ∪ equation_list_var_set ES :=
-  by
-  unfold equation_list_var_set
-  unfold equation_list_formula_list
-  simp only [formula_list_var_set]
-  simp only [Equation.var_set]
-  simp only [List.foldr_cons, Finset.union_assoc]
+-------------------------------------------------------------------------------
+
+
+-- lemma var_occurs_in_equation_list_iff_mem_equation_list_var_set
+
+-- lemma var_occurs_in_equation_list_iff_mem_equation_list_var_list
 
 
 -------------------------------------------------------------------------------
@@ -271,7 +323,6 @@ def equation_replace_var_one_rec
   ⟨replace_var_one_rec X F E.lhs, replace_var_one_rec X F E.rhs⟩
 
 
-
 /--
   `equation_list_replace_var_one_rec X F ES` :=
 
@@ -287,4 +338,17 @@ def equation_list_replace_var_one_rec
   ES.map (fun (E : Equation) => equation_replace_var_one_rec X F E)
 
 
-#lint
+example
+  (X : String)
+  (F : Formula_)
+  (ES : List Equation)
+  (h1 : X ∉ equation_list_var_set ES) :
+  equation_list_replace_var_one_rec X F ES = ES :=
+  by
+  unfold equation_list_replace_var_one_rec
+  apply List.fun_is_id_on_mem_imp_map_eq_self
+  intro E a1
+  sorry
+
+
+--#lint
